Split IsPure into IntoPure and FromPure.
This tweak allows us to declare pvs as an instance of FromPure (it is not
an instance of IntoPure), making some tactics (like iPureIntro and done)
work with pvs too.

proofmode/classes.v
@@ -17,15 +17,24 @@ Global Instance from_assumption_always_r P Q :
   FromAssumption true P Q → FromAssumption true P (□ Q).
 Proof. rewrite /FromAssumption=><-. by rewrite always_always. Qed.
 
-Class IsPure (P : uPred M) (φ : Prop) := is_pure : P ⊣⊢ ■ φ.
-Global Arguments is_pure : clear implicits.
-Global Instance is_pure_pure φ : IsPure (■ φ) φ.
+Class IntoPure (P : uPred M) (φ : Prop) := into_pure : P ⊢ ■ φ.
+Global Arguments into_pure : clear implicits.
+Global Instance into_pure_pure φ : IntoPure (■ φ) φ.
 Proof. done. Qed.
-Global Instance is_pure_eq {A : cofeT} (a b : A) :
-  Timeless a → IsPure (a ≡ b) (a ≡ b).
-Proof. intros; red. by rewrite timeless_eq. Qed.
-Global Instance is_pure_valid `{CMRADiscrete A} (a : A) : IsPure (✓ a) (✓ a).
-Proof. intros; red. by rewrite discrete_valid. Qed.
+Global Instance into_pure_eq {A : cofeT} (a b : A) :
+  Timeless a → IntoPure (a ≡ b) (a ≡ b).
+Proof. intros. by rewrite /IntoPure timeless_eq. Qed.
+Global Instance into_pure_valid `{CMRADiscrete A} (a : A) : IntoPure (✓ a) (✓ a).
+Proof. by rewrite /IntoPure discrete_valid. Qed.
+
+Class FromPure (P : uPred M) (φ : Prop) := from_pure : φ → True ⊢ P.
+Global Arguments from_pure : clear implicits.
+Global Instance from_pure_pure φ : FromPure (■ φ) φ.
+Proof. intros ?. by apply pure_intro. Qed.
+Global Instance from_pure_eq {A : cofeT} (a b : A) : FromPure (a ≡ b) (a ≡ b).
+Proof. intros ->. apply eq_refl. Qed.
+Global Instance from_pure_valid {A : cmraT} (a : A) : FromPure (✓ a) (✓ a).
+Proof. intros ?. by apply valid_intro. Qed.
 
 Class IntoPersistentP (P Q : uPred M) := into_persistentP : P ⊢ □ Q.
 Global Arguments into_persistentP : clear implicits.
